src/Init/Data/BitVec/Bitblast.lean
@@ -631,6 +631,7 @@ A recurrence that describes multiplication as repeated addition.
 
 This function is useful for bit blasting multiplication.
 -/
+@[expose]
 def mulRec (x y : BitVec w) (s : Nat) : BitVec w :=
   let cur := if y.getLsbD s then (x <<< s) else 0
   match s with
@@ -1091,6 +1092,7 @@ theorem lawful_divSubtractShift (qr : DivModState w) (h : qr.Poised args) :
 /-! ### Core division algorithm circuit -/
 
 /-- A recursive definition of division for bit blasting, in terms of a shift-subtraction circuit. -/
+@[expose]
 def divRec {w : Nat} (m : Nat) (args : DivModArgs w) (qr : DivModState w) :
     DivModState w :=
   match m with
