src/Init/GetElem.lean
@@ -293,12 +293,12 @@ instance : GetElem (List α) Nat α fun as i => i < as.length where
   getElem as i h := as.get ⟨i, h⟩
 
 @[simp, grind]
-theorem getElem_cons_zero (a : α) (as : List α) (h : 0 < (a :: as).length) : getElem (a :: as) 0 h = a := by
-  rfl
+theorem getElem_cons_zero (a : α) (as : List α) (h : 0 < (a :: as).length) :
+    getElem (a :: as) 0 h = a := rfl
 
 @[simp, grind]
-theorem getElem_cons_succ (a : α) (as : List α) (i : Nat) (h : i + 1 < (a :: as).length) : getElem (a :: as) (i+1) h = getElem as i (Nat.lt_of_succ_lt_succ h) := by
-  rfl
+theorem getElem_cons_succ (a : α) (as : List α) (i : Nat) (h : i + 1 < (a :: as).length) : getElem (a :: as) (i+1) h = getElem as i (Nat.lt_of_succ_lt_succ h) :=
+    rfl
 
 @[simp, grind] theorem getElem_mem : ∀ {l : List α} {n} (h : n < l.length), l[n]'h ∈ l
   | _ :: _, 0, _ => .head ..
